Work on monads

Monads.lean
@@ -1,102 +1,18 @@
 
-abbrev ℕ := Nat
+def unit_left (m : Type u → Type v) [Monad m] :=
+  ∀ {α β : Type u}, ∀ {f : α -> m β}, (fun a => (a |> pure) >>= f) = f
+  -- or (pure · >>= f) = f
 
-def randRange₀ (n : Nat) : Nat :=
-  sorry
+def unit_left' (m : Type u → Type v) [Monad m] :=
+  ∀ {α β : Type u}, ∀ {f : α -> m β}, pure >=> f = f
 
-theorem reflexivity : ∀ (r : ℕ), r = r := by
-  intro r
-  rfl
+theorem ul' (m : Type u → Type v) [Monad m] : unit_left m -> unit_left' m := by
+  intro h
+  intro α β f
+  ext x
+  rw [Bind.kleisliRight]
+  rw [unit_left] at h
+  exact congrFun (h (f := f)) x
 
-theorem rand_theorem (n : Nat) : randRange₀ n = randRange₀ n :=
-  reflexivity (randRange₀ n)
-
--- So .... we are only going to be able to have constant random numbers with
--- this signature !!!
-
-def randRange (n : Nat) : IO Nat :=
-  IO.Process.run {
-    cmd := "python",
-    args := #[
-      "-c",
-      s!"import random; print(random.randrange(0, {n}), end='')"
-    ]
-  } >>= (· |> String.toNat! |> pure)
-
-
-#eval "0x" ++ String.mk (Nat.toDigits 16 255)
-
-def hex₀ (n : Nat) : String :=
-  "0x" ++ String.mk (Nat.toDigits 16 n)
-
-def hex₁ (n : Nat) : String :=
-  n |> fun n => Nat.toDigits 16 n |> String.mk |> fun s => "0x" ++ s
-
-#eval hex₁ 42
--- "0x2a"
-
-def hex₂ (n : Nat) : String :=
-  n |> Nat.toDigits 16 |> String.mk |> ("0x" ++ ·)
-
-def hex := hex₁
-
-
-#eval hex 0
--- "0x0"
-
-#eval hex 42
--- "0x2a"
-
-#eval hex 255
--- "0xff"
-
-#eval hex 4096
--- "0x1000"
-
-def a := {
-  cmd := "python3", args := #["-c"]
-  : IO.Process.SpawnArgs
-}
-
-def strip_python (s : String) : IO String :=
-  let python_code := s!"print('{s}'.strip(), end='')"
-  let spawnArgs : IO.Process.SpawnArgs := {
-    cmd := "python", args := #["-c", python_code]
-  }
-  IO.Process.run spawnArgs
-
-#eval strip_python "  Hello world!  "
--- "Hello world!"
-
-#eval strip_python "0x42\n"
--- process 'python' exited with code 1 !
-
-def hex_python₀ (n : Nat) : IO String :=
-  let python_code := s!"print(hex({n}))"
-  let spawnArgs : IO.Process.SpawnArgs := {
-    cmd := "python", args := #["-c", python_code]
-  }
-  IO.Process.run spawnArgs >>= strip_python
-
-#eval hex_python₀
--- "0x2a"
-
-def hex_python₉  (n : Nat) : IO String := do
-  let python_code := s!"print(hex({n}))"
-  let spawnArgs := { cmd := "python3", args := #["-c", python_code] }
-  let out ← IO.Process.run spawnArgs
-  return out.trim
-
-#eval hex_python 42
-
-def one_plus_one_python : IO String := do
-  let spawnArgs := { cmd := "python3", args := #["-c", "print(1+1)"] }
-  let out ←  IO.Process.run spawnArgs
-  return out
-
-def one_plus_one : IO Unit := do
-  let result ← IO.Process.run { cmd := "python3", args := #["-c", "print(1+1)"] }
-  IO.println s!"1 + 1 = {result}"
-
-#eval one_plus_one
--- 1 + 1 = 2
+theorem ul (m : Type u → Type v) [Monad m] : unit_left' m -> unit_left m := by
+  admit
